<script id="MathJax-script" async src="https://cdn.jsdelivr.net/npm/mathjax@3/es5/tex-mml-chtml.js"></script>

1. Prove the following statements:
    \begin{align}
      & \text{(i)} \ \text{If} \ ax = a \ \text{for some number} \ a \neq 0,
      \ \text{then} \ x=1. \\
      & \text{(ii)} \ x^2-y^2 = (x-y)(x+y). \\
      & \text{(iii)} \ \text{If} \ x^2=y^2, \ \text{then} \ x=y \ \text{or}
      \ x=-y. \\
      & \text{(iv)} \ x^3-y^3 = (x-y)(x^2 + xy + y^2). \\
      & \text{(v)} \ x^n-y^n = (x-y)(x^{n-1} + x^{n-2}y + \dots + xy^{n-2}
      + y^{n-1}).
    \end{align}

2. What is wrong with the following "proof"? Let \(x = y\). Then
	\begin{equation}
	  \begin{split}
	    x^2 &= xy, \\
	    x^2-y^2 &= xy-y^2, \\
	    (x+y)(x-y) &= y(x-y), \\
	    x+y &= y, \ \ \ \color{grey}{\text{Division by zero is undefined}} \\
	    2y &= y, \\
	    2 &= 1. \\
	    & \ \square
	  \end{split}
	\end{equation}

3. Prove the following:
	\begin{array}{ll}
	  \text{(i)} & \dfrac{a}{b} = \dfrac{ac}{bc}, \ \text{if} \ b,c \neq 0. \\
	  \text{(ii)} & \dfrac{a}{b} + \dfrac{c}{d} = \dfrac{ad+bc}{bd}, \ \text{if}
	  \ b,d \neq 0. \\
	  \text{(iii)} & (ab)^{-1}=a^{-1}b^{-1}, \ \text{if} \ a,b \neq 0. \
	  \text{(To do this, you must} \\
	  & \text{remember the defining property of} \ (ab)^{-1}). \\
	  \text{(iv)} & \dfrac{a}{b} \cdot \dfrac{c}{d} = \dfrac{ac}{db}, \
	  \text{if} \ b,d \neq 0. \\
	  \text{(v)} & \dfrac{a}{b} \bigg/ \dfrac{c}{d} = \dfrac{ad}{bc}, \
	  \text{if} \ b,c,d \neq 0. \\
	  \text{(vi)} & \text{If} \ b,d \neq 0, \ \text{then} \ \dfrac{a}{b} =
	  \dfrac{c}{d}, \ \text{if and only if} \ ad=bc. \ \text{Also determine} \\
	  & \text{when} \ \dfrac{a}{b} = \dfrac{b}{a}.
	\end{array}
